\documentclass[12pt]{article}
\usepackage{amsmath}

\begin{document}

\[
f(a,b) = \sum_{i=1}^n (y_i - a - b x_i)^2
\]

\begin{enumerate}
  \item function $f$ partial derivative $a$ï¼š
  
  use chain rule
  
  \[
    \frac{\partial f}{\partial a} = -2 \sum_{i=1}^n (y_i - a - b x_i)
  \]

  \item function $f$ partial derivative $b$: 
  
  use chain rule
  
  \[
    \frac{\partial f}{\partial b} = -2 \sum_{i=1}^n (y_i - a - b x_i) x_i
  \]

  \item solve $(a,b)$:
  \[
    \begin{cases}
        \frac{\partial f}{\partial a} = 0 
        \implies\sum_{i=1}^n (y_i - a - b x_i) = 0
         \\[2mm]
        \frac{\partial f}{\partial b} = 0 \implies \sum_{i=1}^n (y_i - a - b x_i)x_i = 0
        \\[1mm]
        \end{cases}
    \]
  
there is trivial if we assume that
   \[
    \bar{y} = \frac{\sum_{i = 1}^n(y_i)}{n},
    \bar{x} = \frac{\sum_{i = 1}^n(x_i)}{n}
   \]
   
    \[ \implies  a = \bar{y} - b \bar{x},\]

   to slove $\frac{\partial f}{\partial b} = 0$ we substitute result $a = \bar{y} - b \bar{x}$
     \[
        a = \bar{y} - b \bar{x}
     \implies \sum_{i=1}^n (y_i - (\bar{y}-b\bar{x}) - b x_i)x_i = 0 
     \]
     in further,
     \[
     b = \frac{\sum(y_i - \bar{y})x_i}{\sum(x_i - \bar{x})x_i}
     \]
     notice that \[\sum{\bar{x}x_i} = n\bar{x}^2 , \sum{\bar{y}x_i} = n\bar{x}\bar{y} \]
 \[ b = \frac{\sum{x_iy_i-2n\bar{x}\bar{y}}+n\bar{x}\bar{y}}{\sum{x_i^2-2n\bar{x}^2}+n\bar{x}^2} \]   
 use Binomial Theorem

    \[\implies b = \frac{\sum_{i=1}^n (x_i - \bar{x})(y_i - \bar{y})}{\sum_{i=1}^n (x_i - \bar{x})^2}
        \]
    \[\implies
    \begin{cases}
    
    a = \bar{y} - b \bar{x}, \\[2mm]
        
    b = \frac{\sum(x_i - \bar{x})(y_i - \bar{y})}{\sum (x_i - \bar{x})^2}
        \end{cases}
    \]
\end{enumerate}

\end{document}
